cryptis/core/pre_term/with_stdpp.v
@@ -82,6 +82,7 @@ Instance repr_term_op2 : Repr term_op2 := λ o,
   match o with
   | O2Pair => #0
   | O2Seal => #1
+  | O2Exp => #TExpOp_tag
   end.
 
 Section ValOfPreTerm.
@@ -96,8 +97,8 @@ Definition val_of_pre_term : Repr pre_term := fix val_of_pre_term pt :=
     (#TOp1_tag, (repr o, val_of_pre_term t))%V
   | PT2 o t1 t2 =>
     (#TOp2_tag, (repr o, val_of_pre_term t1, val_of_pre_term t2))%V
-  | PTExp t ts =>
-    (#TExp_tag, (val_of_pre_term t, repr_list (map val_of_pre_term ts)))%V
+  | PTMul ts =>
+    (#TMul_tag, repr_list (map val_of_pre_term ts))%V
   end.
 
 Global Existing Instance val_of_pre_term.
@@ -115,7 +116,7 @@ Fixpoint nonces_of_pre_term pt : gset loc :=
   | PreTerm.PT0 o => nonces_of_term_op0 o
   | PreTerm.PT1 _ t => nonces_of_pre_term t
   | PreTerm.PT2 _ t1 t2 => nonces_of_pre_term t1 ∪ nonces_of_pre_term t2
-  | PreTerm.PTExp t ts => nonces_of_pre_term t ∪ ⋃ map nonces_of_pre_term ts
+  | PreTerm.PTMul ts => ⋃ map nonces_of_pre_term ts
   end.
 
 Global Instance pre_term_inhabited : Inhabited PreTerm.pre_term.
@@ -141,8 +142,8 @@ elim.
 - by move=> o1 t1 IH [] //= o2 t2 [] /repr_term_op1_inj -> /IH ->.
 - move=> o1 t11 IH1 t12 IH2 [] //= o2 t21 t22.
   by move=> [] /repr_term_op2_inj -> /IH1 -> /IH2 ->.
-move=> t1 IHt ts1 IHts [] //= t2 ts2 [] /IHt -> e_ts; congr PreTerm.PTExp.
+move=> ts1 IHts [] //= ts2 [] e_ts; congr PreTerm.PTMul.
 move: e_ts; rewrite repr_list_unseal.
-elim: ts1 IHts ts2 {t1 t2 IHt} => /= [_ [] //|t1 ts1 H [] IHt {}/H IHts].
+elim: ts1 IHts ts2 => /= [_ [] //|t1 ts1 H [] IHt {}/H IHts].
 by case=> //= t2 ts2 [] /IHt -> /IHts ->.
 Qed.
