cryptis/lib/dh.v
@@ -27,6 +27,7 @@ Definition dh_publ t : iProp :=
 
 Definition dh_seed t : iProp :=
   minted t ∧
+  ⌜negb (is_mul t)⌝ ∧
   □ (public t ↔ ▷ False) ∧
   □ (∀ t', exp_pred_base t t' ↔ ▷ □ dh_publ t') ∧
   □ (public (TInv t) ↔ ▷ False) ∧
@@ -37,7 +38,7 @@ Lemma dh_seed_elim0 a :
   public a -∗
   ▷ False.
 Proof.
-iIntros "#(_ & aP & _) #p_t".
+iIntros "#(_ & _ & aP & _) #p_t".
 by iApply "aP".
 Qed.
 
@@ -47,12 +48,13 @@ Lemma dh_seed_exp_pred_base_elim a t :
   exp_pred_base a t -∗
   □ ▷ (⌜t = TExp (base t) a⌝ ∗ P t).
 Proof.
-iIntros "%a_t (_ & _ & #dh & _) #base".
+iIntros "%a_t (_ & _ & _ & #dh & _) #base".
 iSpecialize ("dh" with "base"); iModIntro; iNext.
 iDestruct "dh" as "#(%l_t & p_t)"; iFrame "#".
 rewrite -[t in LHS]base_expsK.
 case: (exps t) => // b [|//] in a_t l_t *.
-by rewrite list_elem_of_singleton in a_t; subst b.
+rewrite list_elem_of_singleton in a_t; subst b.
+by rewrite /TExpN TMulN1.
 Qed.
 
 Lemma dh_seed_elim1 g a :
@@ -62,13 +64,17 @@ Lemma dh_seed_elim1 g a :
   ▷ P (TExp g a).
 Proof.
 iIntros "%gNX #aP #p_t".
+iAssert ⌜negb (is_mul a)⌝%I as %Nm_a; first by iDestruct "aP" as "(_ & $ & _)".
 rewrite public_TExp_iff //.
 iDestruct "p_t" as "(_ & _ & p_t & _)".
 set t' := TExp g a.
 (* MOVE *)
 have exps_t': exps t' = [a].
   apply Permutation_singleton_r.
-  by rewrite exps_TExpN exps_expN // cancel_exps1.
+  rewrite /t' (_ : TExp g a = TExpN g [a]); last by rewrite /TExpN TMulN1.
+  rewrite exps_TExpN ?exps_expN //=;
+    [by rewrite cancel_exps1
+    |by rewrite ssrbool.andbT; exact: (proj2 (is_trueP _) Nm_a)].
 (* /MOVE *)
 have a_t' : a ∈ exps t' by rewrite exps_t'; set_solver.
 iPoseProof (exp_pred_inv_same with "p_t") as "[#contra|H]" => //.
@@ -76,7 +82,8 @@ iPoseProof (exp_pred_inv_same with "p_t") as "[#contra|H]" => //.
 iDestruct "H" as "(%t & %e_base & %a_t & H)".
 iDestruct (dh_seed_exp_pred_base_elim with "aP H")
   as "{H} #[>-> H]" => //; iNext.
-by rewrite -{2}[t']base_expsK exps_t' e_base.
+have -> : t' = TExp (base t) a; last by iApply "H".
+by rewrite /t' e_base base_TExp base_expN.
 Qed.
 
 Lemma dh_seed_elim2 g a b :
@@ -89,8 +96,14 @@ Lemma dh_seed_elim2 g a b :
   ▷ False.
 Proof.
 iIntros "%gXN %a_b %a_bV #aP #bP #p".
+iAssert ⌜negb (is_mul a)⌝%I as %Nm_a; first by iDestruct "aP" as "(_ & $ & _)".
+iAssert ⌜negb (is_mul b)⌝%I as %Nm_b; first by iDestruct "bP" as "(_ & $ & _)".
 have exps_t : exps (TExpN g [a; b]) ≡ₚ [a; b].
-  by rewrite exps_TExpN exps_expN //= cancel_exps_canceled ?invs_canceled2.
+  rewrite exps_TExpN ?exps_expN //=.
+  - by rewrite (cancel_exps_canceled
+      (proj2 (invs_canceled2 (proj2 (is_trueP _) Nm_a)
+                             (proj2 (is_trueP _) Nm_b)) a_bV)).
+  - by rewrite (proj2 (is_trueP _) Nm_a) (proj2 (is_trueP _) Nm_b).
 have a_t : a ∈ exps (TExpN g [a; b]) by rewrite exps_t; set_solver.
 have b_t : b ∈ exps (TExpN g [a; b]) by rewrite exps_t; set_solver.
 iPoseProof (exp_pred_exps a_t with "p") as "[dh_a _]".
@@ -103,11 +116,12 @@ iDestruct "p_c" as "[p_c|(%t' & %ebase & %exps_t'S & contra)]".
   - iDestruct (dh_seed_elim0 with "bP p_c") as ">[]".
 rewrite exps_t in exps_t'S.
 iAssert (▷ □ dh_publ t')%I as "[>%len_t' #H]".
-  iDestruct "aP" as "(_ & _ & #aP & _)".
-  iDestruct "bP" as "(_ & _ & #bP & _)".
+  iDestruct "aP" as "(_ & _ & _ & #aP & _)".
+  iDestruct "bP" as "(_ & _ & _ & #bP & _)".
   by case: c_t => ->; [iApply "aP"|iApply "bP"].
 case exps_t': (exps t') => [//|d [|//]] in exps_t'S len_t'.
-have ->: t' = TExp g d by rewrite -exps_t' -ebase base_expsK.
+have ->: t' = TExp g d.
+  by rewrite -[t' in LHS]base_expsK ebase exps_t' /TExpN TMulN1.
 move: a_b.
 have /list_elem_of_singleton ->: a ∈ [d] by set_solver.
 have /list_elem_of_singleton ->: b ∈ [d] by set_solver.
@@ -121,10 +135,15 @@ Lemma dh_public_TExp g a :
   ▷ □ P (TExp g a) -∗
   public (TExp g a).
 Proof.
-iIntros "%gXN #gP (#m & #aP1 & #aP2 & #aPV & _) #P_a".
+iIntros "%gXN #gP (#m & %Nm_a & #aP1 & #aP2 & #aPV & _) #P_a".
 rewrite public_TExp_iff //; do !iSplit => //.
 - iApply exp_pred_intro1. iApply "aP2"; do 2!iModIntro; iSplit => //.
-  by rewrite exps_TExpN exps_expN.
+  iPureIntro; suff -> : exps (TExp g a) = [a] by [].
+  apply Permutation_singleton_r.
+  rewrite (_ : TExp g a = TExpN g [a]); last by rewrite /TExpN TMulN1.
+  rewrite exps_TExpN ?exps_expN //=;
+    [by rewrite cancel_exps1
+    |by rewrite ssrbool.andbT; exact: (proj2 (is_trueP _) Nm_a)].
 - iModIntro; iIntros "#p".
   by iApply False_public; last iApply "aPV".
 Qed.
@@ -156,10 +175,11 @@ iApply (wp_mk_nonce_freshN T (λ _, False%I) dh_publ
   - rewrite minted_TExp //; iIntros "!>"; iSplit; eauto.
     by iIntros "[??]".
 iIntros (a) "%a_T %nonce_a #m_a #aP #? #sV #? token".
+have Nm_a : negb (is_mul a) by case: (a) nonce_a.
 have a_g: TInv a ∉ exps g.
   by rewrite exps_expN // elem_of_nil; case.
-have [? [] aV_ga a_ga] := tsize_lt_TExp a_g.
-have {}a_aV : TInv a ≠ a := @TInv_neq a.
+have [? [] aV_ga a_ga] := tsize_lt_TExp Nm_a a_g.
+have {}a_aV : TInv a ≠ a := TInv_neq Nm_a.
 have {}a_ga : a ≠ TExp g a.
   move=> contra; rewrite -contra in a_ga; lia.
 have {}aV_ga : TInv a ≠ TExp g a.
